Nemonuri/SequenceProd/Basic.lean
@@ -98,6 +98,15 @@ def head? (sp: SequenceProd α β) : OptionProd α β :=
   | .none, .some x => .snd x
   | .none, .none => .none
 
+theorem head?_eq_ofProd? : sp.head? = OptionProd.ofProd? (sp.fst.head?, sp.snd.head?) := by
+  rw [← OptionProd.equivOfProd?.symm.injective.eq_iff]
+  simp
+  rw [OptionProd.leftInverse_toProd?_ofProd? _]
+  dsimp [head?]
+  split <;> rename_i lm1 lm2 <;> simp [OptionProd.toProd?, lm1, lm2]
+
+
+
 def head (sp: SequenceProd α β) (req1: sp.toEmptyLabelEq = .eq) (req2: sp.toEmptyLabel req1 = .nonempty) : Prod α β :=
   have lm1 := sp.toEmptyLabel_eq_fst_toEmptyLabel req1 |>.symm.trans req2
   have lm2 := sp.toEmptyLabel_eq_snd_toEmptyLabel req1 |>.symm.trans req2
@@ -114,6 +123,50 @@ theorem head?_eq_ofProd_head (req1: sp.toEmptyLabelEq = .eq) (req2: sp.toEmptyLa
   dsimp [head?]
   simp only [lm1, lm2]
 
+
+def getAt? (sp: SequenceProd α β) (i: ℕ) : OptionProd α β := OptionProd.ofProd? ⟨sp.fst.getAt? i, sp.snd.getAt? i⟩
+
+def getAt (sp: SequenceProd α β) (i: ℕ) (req1: i < sp.fst.length?) (req2: i < sp.snd.length?) : Prod α β := ⟨sp.fst.getAt i req1, sp.snd.getAt i req2⟩
+
+theorem getAt?_eq_ofProd_getAt {i: ℕ} (req1: i < sp.fst.length?) (req2: i < sp.snd.length?)
+  : sp.getAt? i = OptionProd.ofProd (sp.getAt i req1 req2) := by
+  dsimp [getAt]
+  dsimp [getAt?]
+  rw [← OptionProd.equivOfProd?.symm.injective.eq_iff]
+  simp only [OptionProd.equivOfProd?_symm_apply]
+  rw [OptionProd.leftInverse_toProd?_ofProd? _]
+  dsimp [OptionProd.toProd?]
+  rw [Prod.ext_iff]
+  dsimp
+  refine And.intro ?_ ?_
+  · exact Sequence.getAt?_eq_some_getAt req1
+  · exact Sequence.getAt?_eq_some_getAt req2
+
+
+def getAt?Flip (i: ℕ) {α β: Type _} (sp: SequenceProd α β) : OptionProd α β := sp.getAt? i
+
+@[defeq]
+theorem getAt?Flip_eq_getAt? {i: ℕ} : getAt?Flip i sp = sp.getAt? i := rfl
+
+theorem head?_eq_getAt?Flip_zero : @head? = @getAt?Flip 0 := by
+  ext α β sp
+  dsimp [getAt?Flip_eq_getAt?]
+  dsimp [getAt?]
+  simp only [← Sequence.head?_eq_getAt?_zero]
+  refine OptionProd.ext ?_ ?_
+  · simp only [OptionProd.ofProd?_fst?]
+    dsimp [head?]
+    split <;> rename_i lm1 _ <;> simp [lm1]
+  · simp only [OptionProd.ofProd?_snd?]
+    dsimp [head?]
+    split <;> rename_i _ lm2 <;> simp [lm2]
+
+def getFromEndAt? (sp: SequenceProd α β) (i: ℕ) (sentinel?: OptionProd α β) : OptionProd α β :=
+  let x := sentinel?.toProd?
+  OptionProd.ofProd? ⟨sp.fst.getFromEndAt? i x.fst, sp.snd.getFromEndAt? i x.snd⟩
+
+def getFromLastAt? (sp: SequenceProd α β) (i: ℕ) : OptionProd α β :=
+  OptionProd.ofProd? ⟨sp.fst.getFromLastAt? i, sp.snd.getFromLastAt? i⟩
 
 end SequenceProd
 
