Nemonuri/SequenceProd/Operations.lean
@@ -33,16 +33,63 @@ theorem singleFst_toFinLabel {a: α} : (singleFst α β a).toFinLabel singleFst_
 def stepL (a: α) (b: β) : SequenceProd α β → SequenceProd α β
   | ⟨fst, snd⟩ => ⟨Sequence.cons a fst, Sequence.cons b snd⟩
 
-theorem stepL_toEmptyLabelEq : (sp.stepL a b).toEmptyLabelEq = .eq := by
+theorem stepL_emptyLabel_eq : (sp.stepL a b).toEmptyLabelEq = .eq := by
   rw [toEmptyLabel_eq_eq_iff]
   dsimp [stepL]
   simp only [Sequence.cons_nonempty]
 
-theorem stepL_toEmptyLabel : (sp.stepL a b).toEmptyLabel stepL_toEmptyLabelEq = .nonempty := by
+theorem stepL_nonempty : (sp.stepL a b).toEmptyLabel stepL_emptyLabel_eq = .nonempty := by
   rw [toEmptyLabel_eq_fst_toEmptyLabel]
   dsimp [stepL]
   simp only [Sequence.cons_nonempty]
 
+theorem stepL_head? : (sp.stepL a b).head? = OptionProd.both a b := by
+  rw [head?_eq_ofProd?]
+  refine OptionProd.ext ?_ ?_
+  <;> (simp; dsimp [stepL]; exact cons_head?)
+
+theorem stepL_head : (sp.stepL a b).head stepL_emptyLabel_eq stepL_nonempty = (a, b) := by
+  rw [← OptionProd.ofProd_injective.eq_iff]
+  rw [← SequenceProd.head?_eq_ofProd_head]
+  refine stepL_head?.trans ?_
+  dsimp
+
+
+def tail : SequenceProd α β → SequenceProd α β
+  | ⟨fst, snd⟩ => ⟨fst.tail, snd.tail⟩
+
+theorem stepL_tail : (sp.stepL a b).tail = sp := by
+  refine SequenceProd.ext ?_ ?_
+  <;> dsimp [tail, stepL]
+  <;> rw [← Sequence.ext_iff]
+  <;> exact Sequence.cons_tail
+
+/-
+theorem stepL_eta (req1: sp.toEmptyLabelEq = .eq) (req2: sp.toEmptyLabel req1 = .nonempty)
+  : let x := sp.head req1 req2; stepL x.fst x.snd sp.tail = sp := by
+  extract_lets x
+  rcases lm1: x with ⟨a, b⟩
+  subst x
+  dsimp
+  rewrite [Prod.ext_iff] at lm1
+  rcases lm1 with ⟨lm1, lm2⟩
+  dsimp at lm1 lm2
+  refine SequenceProd.ext ?_ ?_
+  <;> rw [← Sequence.ext_iff]
+  <;> dsimp [tail, stepL]
+  <;> rw [Sequence.tail_cons_eq_self_iff]
+  · refine Exists.intro ?_ ?_
+    ·
+-/
+
+
+/-
+theorem stepL_head : (sp.stepL a b).head stepL_toEmptyLabelEq stepL_toEmptyLabel = (a, b) := by
+  dsimp [head]
+  refine Prod.ext ?_ ?_ <;>
+  dsimp [stepL]
+  exact Sequence.cons_head?
+-/
 
 end Nemonuri.SequenceProd
 
